ReducibilityCandidate.v
@@ -1,0 +1,60 @@
+Require Import Termination.Syntax.
+Require Import Termination.Sets.
+Require Import Termination.Tactics.
+Require Import Termination.SmallStep.
+Require Import Termination.AssocList.
+
+Require Import PeanoNat.
+
+Open Scope list_scope.
+
+Definition reducibility_candidate (P: term -> Prop): Prop :=
+  forall v, P v -> is_value v /\ wf v 0 /\ pfv v term_var = nil.
+
+(* an interpretation for every type variable, as a reducibility candidate *)
+Definition interpretation: Type := list (nat * (term -> Prop)).
+
+Fixpoint valid_interpretation (theta: interpretation): Prop :=
+  match theta with
+  | nil => True
+  | (x,P) :: theta' => valid_interpretation theta' /\ reducibility_candidate P
+  end.
+
+Lemma in_valid_interpretation_closed: forall theta v X P,
+  valid_interpretation theta ->
+  lookup Nat.eq_dec theta X = Some P ->
+  P v ->
+  (is_value v /\ wf v 0 /\ pfv v term_var = nil).
+Proof.
+  induction theta as [ | p theta' IH ]; repeat unfold reducibility_candidate in * || step;
+    eauto;
+    try solve [ apply_any; steps ];
+    try solve [ eapply IH; steps; eauto ].
+Qed.
+
+Lemma in_valid_interpretation_fv: forall theta v X P,
+  valid_interpretation theta ->
+  lookup Nat.eq_dec theta X = Some P ->
+  P v ->
+  pfv v term_var = nil.
+Proof.
+  induction theta; repeat step || eauto || apply_any.
+Qed.
+
+Lemma in_valid_interpretation_wf: forall theta v X P,
+  valid_interpretation theta ->
+  lookup Nat.eq_dec theta X = Some P ->
+  P v ->
+  wf v 0.
+Proof.
+  induction theta; repeat step || eauto || apply_any.
+Qed.
+
+Lemma in_valid_interpretation_value: forall theta v X P,
+  valid_interpretation theta ->
+  lookup Nat.eq_dec theta X = Some P ->
+  P v ->
+  is_value v.
+Proof.
+  induction theta; repeat step || eauto || apply_any.
+Qed.
