ReducibilitySetOpsRules.v
@@ -26,6 +26,7 @@ Require Import Termination.FVLemmasLists.
 Require Import Termination.WFLemmas.
 Require Import Termination.WFLemmasLists.
 
+Require Import Termination.ReducibilityCandidate.
 Require Import Termination.ReducibilityDefinition.
 Require Import Termination.ReducibilityLemmas.
 Require Import Termination.ReducibilityLetRules.
