ReducibilitySplitMatchRule.v
@@ -30,6 +30,7 @@ Require Import Termination.SetLemmas.
 Require Import Termination.Equivalence.
 Require Import Termination.EquivalenceLemmas.
 
+Require Import Termination.ReducibilityCandidate.
 Require Import Termination.ReducibilityDefinition.
 Require Import Termination.ReducibilityLemmas.
 Require Import Termination.RedTactics.
